\documentclass{article}
\usepackage{epsfig}
\usepackage{amsmath}
\usepackage{amssymb}
\pagestyle{empty}
\begin{document}
\[ f_j= \sum_{k=-\frac{N}{2}}^{\frac{N}{2}-1} \hat{f}_{k} {\rm e}^{2\pi{\rm i}\frac{kj}{N}} \]
\pagebreak

$j=-\frac{N}{2},\dots,\frac{N}{2}-1$
\pagebreak

$\hat{f}_{k}\in\mathbb{C}$
\pagebreak

${\cal O}(N^2)$
\pagebreak

${\cal O}(N\log N)$
\pagebreak

$\mathbf{k}\in\mathbb{Z}^d$
\pagebreak

\[ I_{\mathbf{N}} := \left\{ \mathbf{k}=\left(k_t\right)_{t=0,\dots,d-1} \in \mathbb{Z}^d: - \frac{N_t}{2} \le k_t < \frac{N_t}{2} ,\;t=0,\dots,d-1\right\}, \]
\pagebreak

$\mathbf{N}=\left(N_t\right)_{t=0,\dots,d-1}$
\pagebreak

$N_t\in 2\mathbb{N}$
\pagebreak

$\hat f_{\mathbf{k}} \in \mathbb{C}$
\pagebreak

$\mathbf{k}\in I_{\mathbf{N}}$
\pagebreak

\[ f\left(\mathbf{x}\right) := \sum_{ \mathbf{k}\in I_{ N}} \hat{f}_{\mathbf{ k}} {\rm e}^{-2\pi{\rm i}\mathbf{k}\mathbf{ x}} \]
\pagebreak

$\mathbf{x}_j \in \mathbb{T}^d$
\pagebreak

$j=0,\ldots, M-1$
\pagebreak

$ d$
\pagebreak

\[ \hat h_{\mathbf{k}} := \sum_{j=0}^{M-1} {f}_{j} {\rm e}^{2\pi{\rm i}\mathbf{k}\mathbf{ x}_j}. \]
\pagebreak

$M \in \mathbb{N}_0$
\pagebreak

$m \in \mathbb{N}_0$
\pagebreak

$m = 0,\ldots,M$
\pagebreak

$M+1$
\pagebreak

$t \in \mathbb{N}, t \ge 2$
\pagebreak

$N = 2^t \in \mathbb{N}, N \ge 4$
\pagebreak

$m \in \mathbb{N}, 0 \le m \le M$
\pagebreak

$\alpha_k \in \mathbb{R}$
\pagebreak

$k=0,\ldots,N$
\pagebreak

$=\alpha_k$
\pagebreak

$\beta_k \in \mathbb{R}$
\pagebreak

$=\beta_k$
\pagebreak

$\gamma_k \in \mathbb{R}$
\pagebreak

$=\gamma_k$
\pagebreak

$k_{\text{start}} \in \mathbb{N}_0, 0 \le k_{\text{start}} \le N$
\pagebreak

$\kappa \in \mathbb{R}, \kappa > 0$
\pagebreak

$j=0,...,M_{total}-1$
\pagebreak

\[ f(x_j) = \sum_{k \in I_N^2} \hat{f}(k) {\rm e}^{\mbox{\rm\scriptsize i} t_j \omega(k)} {\rm e}^{-2 \pi \mbox{\rm\scriptsize i} k x_j} \]
\pagebreak

$N$
\pagebreak

$x$
\pagebreak

$k \in I_N^2$
\pagebreak

\[ \hat{f}(k) = \sum_{j=0}^{M_{total}-1} f(x_j) {\rm e}^{\mbox{\rm\scriptsize i} t_j \omega(k)} {\rm e}^{-2 \pi \mbox{\rm\scriptsize i} k x_j} \]
\pagebreak

$j=0,...,M\_total-1$
\pagebreak

$f_j^C(x_j) = \sum_{k \in I_0^{N,d}} \hat{f}_k^C * cos(2 \pi k x_j)$
\pagebreak

$k \in I_0^{N,d}$
\pagebreak

$h^C(k) = \sum_{j \in I_0^{(M\_total,1)}} f_j^C * cos(2 \pi k x_j)$
\pagebreak

\[ \mathbb{T}^d := \left\{ \mathbf{x}=\left(x_t\right)_{t=0,\dots,d-1}\in\mathbb{R}^{d}: \; - \frac{1}{2} \le x_t < \frac{1}{2},\; t=0,\dots,d-1 \right\} \]
\pagebreak

$d$
\pagebreak

$\mathbf{x}$
\pagebreak

${\cal X}:=\{\mathbf{x}_j \in {\mathbb T}^d: \,j=0,\dots,M-1\}$
\pagebreak

$\mathbf{k}$
\pagebreak

\[ I_{\mathbf{N}} := \left\{ \mathbf{k}=\left(k_t\right)_{t=0,\dots,d-1}\in \mathbb{Z}^d: - \frac{N_t}{2} \le k_t < \frac{N_t}{2} ,\;t=0,\dots,d-1 \right\}. \]
\pagebreak

\[ f_j = \sum_{\mathbf{k}\in I_{\mathbf{N}}} \hat{f}_{\mathbf{k}} {\rm e}^{-2\pi{\rm i} \mathbf{k}\mathbf{x}_j}, \qquad j=0,\dots,M-1. \]
\pagebreak

\[ \hat f_{\mathbf{k}}=\sum_{j=0}^{M-1} f_j {\rm e}^{+2\pi{\rm i} \mathbf{k}\mathbf{x}_j}, \qquad \mathbf{k}\in I_{\mathbf{N}}. \]
\pagebreak

${\cal O}(|I_{\mathbf{N}}|M)$
\pagebreak

${\cal O}(|I_{\mathbf{N}}|\log|I_{\mathbf{N}}|+M)$
\pagebreak

$\mathbf{D}$
\pagebreak

$\mathbf{B}$
\pagebreak

$(K+1)d$
\pagebreak

$K=2^{10}(m+1)$
\pagebreak

$2dM$
\pagebreak

$(2m+2)dM$
\pagebreak

$(2m+2)^dM$
\pagebreak

$\mathbb{R}^3$
\pagebreak

$(r,\vartheta,\varphi)^{\mathrm{T}}$
\pagebreak

$r \in \mathbb{R}^{+}$
\pagebreak

$\vartheta \in [0,\pi]$
\pagebreak

$\varphi \in [-\pi,\pi)$
\pagebreak

$\mathbb{S}^2$
\pagebreak

\[ \mathbb{S}^2 := \left\{\mathbf{x} \in \mathbb{R}^{3}:\; \|\mathbf{x}\|_2=1\right\} \]
\pagebreak

$(\vartheta,\varphi)^{\mathrm{T}}$
\pagebreak

$x_1 := \frac{\varphi}{2\pi}$
\pagebreak

$x_2 := \frac{\vartheta}{2\pi}$
\pagebreak

$\mathbf{x} := \left(x_1,x_2\right) \in [-\frac{1}{2}, \frac{1}{2}) \times [0,\frac{1}{2}]$
\pagebreak

$P_k : [-1,1] \rightarrow \mathbb{R}$, $k \in \mathbb{N}_{0}$
\pagebreak

\[ P_k(t) := \frac{1}{2^k k!} \frac{\text{d}^k}{\text{d} t^k} \left(t^2-1\right)^k. \]
\pagebreak

\[ (k+1)P_{k+1}(t) = (2k+1) x P_{k}(t) - k P_{k-1}(t) \quad (k \in \mathbb{N}_0). \]
\pagebreak

\[ \left< f,g \right>_{\text{L}^2\left([-1,1]\right)} := \int_{-1}^{1} f(t) g(t) \text{d} t \]
\pagebreak

$\text{L}^2\left([-1,1]\right)$
\pagebreak

\[ \left< P_k,P_l \right>_{\text{L}^2\left([-1,1]\right)} = \frac{2}{2k+1} \delta_{k,l}. \]
\pagebreak

$ c_k := \sqrt{\frac{2k+1}{2}}$
\pagebreak

$c_k P_k$
\pagebreak

\[ \|f\|_{\text{L}^2\left([-1,1]\right)} := \left(<f,f>_{\text{L}^2\left([-1,1]\right)}\right)^{1/2} = \left(\int_{-1}^{1} |f(t)|^2 \; \text{d} t\right)^{1/2}. \]
\pagebreak

$P_k^n : [-1,1] \rightarrow \mathbb{R} $
\pagebreak

$n \in \mathbb{N}_0$
\pagebreak

$k \ge n$
\pagebreak

\[ P_k^n(t) := \left(\frac{(k-n)!}{(k+n)!}\right)^{1/2} \left(1-t^2\right)^{n/2} \frac{\text{d}^n}{\text{d} t^n} P_k(t). \]
\pagebreak

$n = 0$
\pagebreak

$P_k^0 = P_k$
\pagebreak

\[ P_{k+1}^n(t) = v_{k}^n t P_k^n(t) + w_{k}^n P_{k-1}^n(t) \quad (k \ge n), \]
\pagebreak

$P_{n-1}^n(t) := 0$
\pagebreak

$P_{n}^n(t) := \frac{\sqrt{(2n)!}}{2^n n!} \left(1-t^2\right)^{n/2}$
\pagebreak

\[ v_{k}^n := \frac{2k+1}{((k-n+1)(k+n+1))^{1/2}}\; ,\qquad w_{k}^n := - \frac{((k-n)(k+n))^{1/2}}{((k-n+1)(k+n+1))^{1/2}}. \]
\pagebreak

$n$
\pagebreak

$\left\{P_k^n:\: k \ge n\right\}$
\pagebreak

\[ \left< P_k^n,P_l^n \right>_{\text{L}^2\left([-1,1]\right)} = \frac{2}{2k+1} \delta_{k,l} \quad (0 \le n \le k,l). \]
\pagebreak

$ c_k = \sqrt{\frac{2k+1}{2}}$
\pagebreak

$c_k P_k^n$
\pagebreak

$\text{L}^2 \left(\mathbb{S}^2\right)$
\pagebreak

$\tilde{Y}_k^n : \mathbb{S}^2 \rightarrow \mathbb{C}$
\pagebreak

\[ \tilde{Y}_k^n(\vartheta,\varphi) := P_k^{|n|}(\cos\vartheta) \mathrm{e}^{\mathrm{i} n \varphi} \]
\pagebreak

$\text{L}^2\left(\mathbb{S}^2\right)$
\pagebreak

\[ \left< f,g \right>_{\mathrm{L}^2\left(\mathbb{S}^2\right)} := \int_{\mathbb{S}^2} f(\vartheta,\varphi) \overline{g(\vartheta,\varphi)} \: \mathrm{d} \mathbf{\xi} := \int_{-\pi}^{\pi} \int_{0}^{\pi} f(\vartheta,\varphi) \overline{g(\vartheta,\varphi)} \sin \vartheta \; \mathrm{d} \vartheta \; \mathrm{d} \varphi. \]
\pagebreak

$c_k^n := \sqrt{\frac{2k+1}{4\pi}}$
\pagebreak

\[ Y_k^n(\vartheta,\varphi) := c_k^n P_k^{|n|}(\cos\vartheta) \mathrm{e}^{\mathrm{i} n \varphi} \]
\pagebreak

$\text{L}^2\left(\mathbb{S}^2 \right)$
\pagebreak

\[ \|f\|_{\text{L}^2\left(\mathbb{S}^2\right)} = \left(<f,f>_{\text{L}^2\left(\mathbb{S}^2\right)}\right)^{1/2} = \left(\int_{-\pi}^{\pi} \int_{0}^{\pi} |f(\vartheta,\varphi)|^2 \sin \vartheta \; \mathrm{d} \vartheta \; \mathrm{d} \varphi\right)^{1/2}. \]
\pagebreak

$f \in \mathrm{L}^2\left(\mathbb{S}^2\right)$
\pagebreak

\[ f = \sum_{k=0}^{\infty} \sum_{n=-k}^{k} \hat{f}(k,n) Y_k^n, \]
\pagebreak

$\hat{f}(k,n) := \left< f, Y_k^{n} \right>_{\mathrm{L}^2\left(\mathbb{S}^2\right)}$
\pagebreak

$\mathrm{L}^2$
\pagebreak

\[ \begin{array}{rcl} \text{\textbf{Input}} & : & \text{coefficients } \hat{f}(k,n) \in \mathbb{C} \text{ for } k=0,\ldots,N,\;n=-k, \ldots,k,\; N \in \mathbb{N}_0,\\[1ex] & & \text{arbitrary nodes } \mathbf{x}(m) \in [-\frac{1}{2},\frac{1}{2}] \times [0,\frac{1}{2}] \text{ for } m=0,\ldots,M-1, M \in \mathbb{N}. \\[1ex] \text{\textbf{Task}} & : & \text{evaluate } f(m) := f\left( \mathbf{x}(m)\right) = \sum_{k=0}^N \sum_{n=-k}^k \hat{f}_k^n Y_k^n\left(\mathbf{x}(m)\right) \text{ for } m=0,\ldots,M-1. \\[1ex] \text{\textbf{Output}} & : & \text{coefficients } f(m) \in \mathbb{C} \text{ for } m=0,\ldots,M-1.\\ \end{array} \]
\pagebreak

\[ \begin{array}{rcl} \text{\textbf{Input}} & : & \text{coefficients } f(m) \in \mathbb{C} \text{ for } m=0,\ldots,M-1, M \in \mathbb{N},\\ & & \text{arbitrary nodes } \mathbf{x}(m) \in [-\frac{1}{2},\frac{1}{2}] \times [0,\frac{1}{2}] \text{ for } m=0,\ldots,M-1, N \in \mathbb{N}_0.\\[1ex] \text{\textbf{Task}} & : & \text{evaluate } \hat{f}(k,n) := \sum_{m=0}^{M-1} f(m) \overline{Y_k^n\left(\mathbf{x}(m)\right)}cd Do \text{ for } k=0,\ldots,N,\;n=-k,\ldots,k.\\[1ex] \text{\textbf{Output}} & : & \text{coefficients } \hat{f}(k,n) \in \mathbb{C} \text{ for } k=0,\ldots,N,\;n=-k,\ldots,k.\\[1ex] \end{array} \]
\pagebreak

$N \in \mathbb{N}_0$
\pagebreak

$ = (2N+2)^2$
\pagebreak

$M$
\pagebreak

$(2N+2)^2$
\pagebreak

$i \in \mathbb{N}_0$
\pagebreak

$i$
\pagebreak

$i=0,1,\ldots,(2N+2)^2-1$
\pagebreak

$\hat{f}(k,n)$
\pagebreak

$0 \le k \le M$
\pagebreak

$-k \le n \le k$
\pagebreak

$i = (N+2)(N-n+1)+N+k+1$
\pagebreak

$k,n$
\pagebreak

$f(m)$
\pagebreak

$m=0,\ldots,M-1$
\pagebreak

$m$
\pagebreak

$\mathbf{x}(m) \in [-\frac{1}{2},\frac{1}{2}] \times [0,\frac{1}{2}]$
\pagebreak

$m = 0, \ldots,M-1$
\pagebreak

$2m$
\pagebreak

$x_1$
\pagebreak

$2m+1$
\pagebreak

$x_2$
\pagebreak

$N_{\text{max}}$
\pagebreak

$M \in \mathbb{N}$
\pagebreak

$N \in \mathbb{N}_2$
\pagebreak

$\kappa \in \mathbb{R}^{+}$
\pagebreak

$m = 0,\ldots,M-1$
\pagebreak

\[ f(m) = \sum_{k=0}^N \sum_{n=-k}^k \hat{f}(k,n) Y_k^n\left(2\pi x_1(m), 2\pi x_2(m)\right). \]
\pagebreak

$k=0,\ldots,N; n=-k,\ldots,k$
\pagebreak

\[ \hat{f}(k,n) = \sum_{m = 0}^{M-1} f(m) Y_k^n\left(2\pi x_1(m), 2\pi x_2(m)\right). \]
\pagebreak

\[ \tilde{Y}_k^n(\vartheta,\varphi) = P_k^{|n|}(\cos\vartheta) \mathrm{e}^{\mathrm{i} n \varphi}. \]
\pagebreak

$L_2$
\pagebreak

\[ Y_k^n(\vartheta,\varphi) = \sqrt{\frac{2k+1}{4\pi}} P_k^{|n|}(\cos\vartheta) \mathrm{e}^{\mathrm{i} n \varphi}. \]
\pagebreak

$f_hat(k,n)$
\pagebreak

$0 \le k \le N$
\pagebreak

\[ (N+2)(N-n+1)+N+k+1 \]
\pagebreak

\[ f(g_m) = \sum_{l=0}^B \sum_{m=-l}^l \sum_{n=-l}^l \hat{f}^{mn}_l D_l^{mn}\left( \alpha_m,\beta_m,\gamma_m\right). \]
\pagebreak

$l=0,\ldots,B; m,n=-l,\ldots,l$
\pagebreak

\[ \hat{f}^{mn}_l = \sum_{m = 0}^{M-1} f(g_m) D_l^{mn}\left( \alpha_m,\beta_m,\gamma_m\right) \]
\pagebreak

\[ D_{mn}^l(\alpha,\beta,\gamma) = d^{mn}_{l}(\cos\beta) \mathrm{e}^{-\mathrm{i} m \alpha}\mathrm{e}^{-\mathrm{i} n \gamma}. \]
\pagebreak

\[ \tilde D_{mn}^l(\alpha,\beta,\gamma) = \sqrt{\frac{2l+1}{8\pi^2}}d^{mn}_{l}(\cos\beta) \mathrm{e}^{-\mathrm{i} m \alpha}\mathrm{e}^{-\mathrm{i} n \gamma} \]
\pagebreak

$\alpha, \beta, \gamma$
\pagebreak

\[ \sum_{m=-l}^l D_{mn}^l(\alpha,\beta,\gamma) Y_m^l(x) = Y_n^l(A^{-1} x) \]
\pagebreak

$f_hat^{mn}_l$
\pagebreak

$l=0,...,B$
\pagebreak

$m,n =-l,...,l$
\pagebreak

$f_j^S(x_j) = \sum_{k \in I_1^{N,d}} \hat{f}_k^S * sin(2 \pi k x_j)$
\pagebreak

$k \in I_1^{N,d}$
\pagebreak

$h^S(k) = \sum_{j \in I_0^{M\_total,1}} f_j^S * cos(2 \pi k x_j)$
\pagebreak

$v$
\pagebreak

\[ f(x_j) = \sum_{k = 0}^{N_{total}-1} \hat{f}(v_k) {\rm e}^{-2 \pi \mbox{\rm\scriptsize i} v_k x_j \odot N} \]
\pagebreak

$k=0,...,N_{total}-1$
\pagebreak

\[ \hat{f}(v_k) = \sum_{j = 0}^{M_{total}-1} f(x_j) {\rm e}^{2 \pi \mbox{\rm\scriptsize i} v_k x_j \odot N} \]
\pagebreak

\[ \hat{f}(v_k) = \sum_{j = 0}^{M_{tota}l-1} f(x_j) {\rm e}^{2 \pi \mbox{\rm\scriptsize i} v_k x_j \odot N} \]
\pagebreak

$j=0,\dots,M-1$
\pagebreak

\[ f_j = \sum_{k\in H_N^d}\hat f_k {\rm e}^{-2\pi{\rm\scriptsize i}k x_j} \]
\pagebreak

$k\in H_N^d$
\pagebreak

\[ \hat f_k = \sum_{j=0,\dots,M-1} f_j {\rm e}^{+2\pi{\rm\scriptsize i}k x_j} \]
\pagebreak

$x^H x$
\pagebreak

$x^H (w \odot x)$
\pagebreak

$x^H (w\odot w2\odot w2 \odot x)$
\pagebreak

$x^H (w2\odot w2 \odot x)$
\pagebreak

$x \leftarrow y$
\pagebreak

$x \leftarrow a y$
\pagebreak

$x \leftarrow w\odot y$
\pagebreak

$x \leftarrow a x + y$
\pagebreak

$x \leftarrow x + a y$
\pagebreak

$x \leftarrow a x + b y$
\pagebreak

$x \leftarrow x + a w\odot y$
\pagebreak

$x \leftarrow a x + w\odot y$
\pagebreak

$[0,1]\times[0,1]{\rm i}$
\pagebreak

$[-1/2,1/2]$
\pagebreak

$2\le\sigma<4$
\pagebreak

$dM$
\pagebreak

$D$
\pagebreak

$N_0+\dots+N_{d-1}$
\pagebreak

$B$
\pagebreak

$\mathbf{x}(m) = \left(x_1,x_2\right) \in [-\frac{1}{2},\frac{1}{2}) \times [0,\frac{1}{2}]$
\pagebreak

$m=0,\ldots, M-1$
\pagebreak

$M \in \mathbb{N},$
\pagebreak

$P_k : \mathbb{R} \rightarrow \mathbb{R}$
\pagebreak

\[ f(x) = \sum_{k=0}^N a_k P_k(x) \quad (N \in \mathbb{N}_0) \]
\pagebreak

\[ P_{k+1}(x) = (alpha_k * x + beta_k)*P_{k}(x) + gamma_k P_{k-1}(x) \quad (alpha_k, beta_k, gamma_k \in \mathbb{R},\; k \ge 0) \]
\pagebreak

$P_{-1}(x) := 0$
\pagebreak

$P_0(x) := \lambda$
\pagebreak

$\left(a_k\right)_{k=0}^N \in \mathbb{C}^{N+1}$
\pagebreak

$\left(x_j\right)_{j=0}^M \in \mathbb{R}^{M+1}$
\pagebreak

$\alpha_{k-1}^n$
\pagebreak

$k,n = 0,1,\ldots,N$
\pagebreak

$(N+1)^2$
\pagebreak

$\beta_{k-1}^n$
\pagebreak

$\gamma_{k-1}^n$
\pagebreak

$P_k^n(x,c)$
\pagebreak

$k$
\pagebreak

$\alpha_c^n,\ldots,\alpha_{c+k}^n$
\pagebreak

$\beta_c^n,\ldots,\beta_{c+k}^n$
\pagebreak

$\gamma_c^n,\ldots,\gamma_{c+k}^n$
\pagebreak

$\left(b_k^n\right)_{k=0}^M$
\pagebreak

$-M \le n \le M$
\pagebreak

\[ f(\cos\vartheta) = \sum_{k=0}^{2\lfloor\frac{M}{2}\rfloor} a_k (\sin\vartheta)^{n\;\mathrm{mod}\;2} T_k(\cos\vartheta) \]
\pagebreak

$\left(c_k^n\right)_{k=0}^M$
\pagebreak

\[ f(\cos\vartheta) = \sum_{k=-M}^{M} c_k \mathrm{e}^{\mathrm{i}k\vartheta} \]
\pagebreak

$n=-M,\ldots,M$
\pagebreak

$\left(b_k^n\right)_{k=0,\ldots,M;n=-M,\ldots,M}$
\pagebreak

$\left(c_k^n\right)_{k=-M,\ldots,M;n=-M,\ldots,M}$
\pagebreak

$\alpha_l^{km}$
\pagebreak

$l$
\pagebreak

$\beta_l^{km}$
\pagebreak

$\gamma_l^{km}$
\pagebreak

$ \alpha_{l}^{km}$
\pagebreak

$ l= 0,\ldots,N $
\pagebreak

$(2N+1)^2(N+1)$
\pagebreak

$ \beta_{l}^{km}$
\pagebreak

$ \gamma_{l}^{km}$
\pagebreak

$ m = -N,\ldots,N $
\pagebreak

$\alpha_{l}^{km}$
\pagebreak

$ k,m = -N,\ldots,N $
\pagebreak

$\beta_{l}^{km}$
\pagebreak

$\gamma_{l}^{km}$
\pagebreak

$d_l^{km}(x,c)$
\pagebreak

$\alpha_c^{km},\ldots,\alpha_{c+l}^{km}$
\pagebreak

$\beta_c^{km},\ldots,\beta_{c+l}^{km}$
\pagebreak

$\gamma_c^{km},\ldots,\gamma_{c+l}^{km}$
\pagebreak

$ d^{km}_l(cos(theta)) $
\pagebreak

$B, B^{\rm T}$
\pagebreak

$\frac{\|x-y\|_{\infty}}{\|x\|_{\infty}} $
\pagebreak

$\frac{\|x-y\|_{\infty}}{\|z\|_1} $
\pagebreak

$\frac{\|x-y\|_2}{\|x\|_2} $
\pagebreak

\[ f(g_q)=\sum^{N}_{l=0}\sum_{m,n=-l}^l \hat f^{mn}_l D_{mn}^l(\alpha_q,\beta_q,\gamma_q) \]
\pagebreak

$[-1/4,1/4]$
\pagebreak

\[ f(y_j) = \sum_{k=1}^N \alpha_k K(x_k-y_j),\quad j=1\dots M. \]
\pagebreak

$I_{n+\alpha}(x)$
\pagebreak

$\mathrm{e}^{-x}$
\pagebreak

$x,alpha$
\pagebreak

$0 \le \alpha < 1$
\pagebreak

$n=0,1,\ldots,nb-1$
\pagebreak

$|x| \ge exparg$
\pagebreak

$\min(nb,0)-1$
\pagebreak

$n=0,1,\ldots,ncalc$
\pagebreak

$J_{\nu}(x)$
\pagebreak

$I_{\nu}(x)$
\pagebreak

$\nu$
\pagebreak

$\varphi_1 \in [-\pi,\pi)$
\pagebreak

$\vartheta_1 \in [0,\pi]$
\pagebreak

$\varphi_2 \in [-\pi,\pi)$
\pagebreak

$\vartheta_2 \in [0,\pi]$
\pagebreak

$\cos \vartheta_1 \cos \vartheta_2 + \sin \vartheta_1 \sin(\vartheta_2 \cos(\varphi_1 - \varphi_2)$
\pagebreak

$Q_h: [-1,1] \rightarrow \mathbb{R}$
\pagebreak

$x \in [-1,1]$
\pagebreak

$h \in (0,1)$
\pagebreak

$Q_h(x)$
\pagebreak

$S_h: [-1,1] \rightarrow \mathbb{R}$
\pagebreak

$S_h(x)$
\pagebreak

$L_{h,\lambda}: [-1,1] \rightarrow \mathbb{R}$
\pagebreak

$\lambda \in \mathbb{N}_0$
\pagebreak

$L_{h,\lambda}(x)$
\pagebreak

$G_\sigma: [-1,1] \rightarrow \mathbb{R}$
\pagebreak

$\sigma \in \mathbb{R}_+$
\pagebreak

$G_\sigma(x)$
\pagebreak

$x_{t,j}$
\pagebreak

$w_{t,j}$
\pagebreak

$T$
\pagebreak

$R$
\pagebreak

\[ x_{t,j} := r_j\left(\cos\theta_t, \sin\theta_t\right)^{\top}\,,\qquad (j,t)^{\top}\in I_{\sqrt{2}R}\times I_T\,. \]
\pagebreak

$r_j$
\pagebreak

$\theta_t$
\pagebreak

$M \approx \frac{4}{\pi}\log(1+\sqrt{2}) T R$
\pagebreak

$(j,t)^{\top}\in I_R\times I_T$
\pagebreak

$r_j := \frac{j}{R} \in [-\frac{1}{2},\frac{1}{2})$
\pagebreak

$\theta_t := \frac{\pi t}{T} \in [-\frac{\pi}{2},\frac{\pi}{2})$
\pagebreak

\[ x_{t,j} := r_j\left(\cos\theta_t, \sin\theta_t\right)^{\top}\,. \]
\pagebreak

$M=TR$
\pagebreak

$j \ne 0$
\pagebreak

\[ w_{t,j} = \frac{\pi}{2TR^2}\left(\left(|j|+\frac{1}{2}\right)^2- \left(|j|-\frac{1}{2}\right)^2\right) = \frac{\pi |j| }{TR^2}\, . \]
\pagebreak

$\frac{1}{2R}$
\pagebreak

$\frac{\pi}{4R^2}$
\pagebreak

$w_{t,0} := \frac{\pi}{4TR^2}$
\pagebreak

$\frac{\pi}{4}(1+\frac{1}{R^2})$
\pagebreak

\[ R_{\theta_t} f\left(\frac{s}{R}\right) = \sum_{r \in I_R} w_r \; \sum_{k \in I_N^2} f_{k} \mathrm{e}^{-2\pi\mathrm{I} k \; (\frac{r}{R}\theta_t)} \, \mathrm{e}^{2\pi\mathrm{i} r s / R} \qquad(t \in I_T, s \in I_R). \]
\pagebreak

$\frac{r}{R}\theta_t$
\pagebreak

$w_r$
\pagebreak

$f_k$
\pagebreak

$t \in T$
\pagebreak

\end{document}
