\documentclass{article}
\usepackage{epsfig}
\usepackage{amsmath}
\usepackage{amssymb}
\pagestyle{empty}
\begin{document}
\[ f_j= \sum_{k=-\frac{N}{2}}^{\frac{N}{2}-1} \hat{f}_{k} {\rm e}^{2\pi{\rm i}\frac{kj}{N}} \]
\pagebreak

$j=-\frac{N}{2},\hdots,\frac{N}{2}-1$
\pagebreak

$\hat{f}_{k}\in\mathbb{C}$
\pagebreak

${\cal O}(N^2)$
\pagebreak

${\cal O}(N\log N)$
\pagebreak

$\mathbf{k}\in\mathbb{Z}^d$
\pagebreak

\[ I_{\mathbf{N}} := \left\{ \mathbf{k}=\left(k_t\right)_{t=0,\hdots,d-1} \in \mathbb{Z}^d: - \frac{N_t}{2} \le k_t < \frac{N_t}{2} ,\;t=0,\hdots,d-1\right\}, \]
\pagebreak

$\mathbf{N}=\left(N_t\right)_{t=0,\hdots,d-1}$
\pagebreak

$N_t\in 2\mathbb{N}$
\pagebreak

$\hat f_{\mathbf{k}} \in \mathbb{C}$
\pagebreak

$\mathbf{k}\in I_{\mathbf{N}}$
\pagebreak

\[ f\left(\mathbf{x}\right) := \sum_{ \mathbf{k}\in I_{ N}} \hat{f}_{\mathbf{ k}} {\rm e}^{-2\pi{\rm i}\mathbf{k}\mathbf{ x}} \]
\pagebreak

$\mathbf{x}_j \in \mathbb{T}^d$
\pagebreak

$j=0,\ldots, M-1$
\pagebreak

$ d$
\pagebreak

\[ \hat h_{\mathbf{k}} := \sum_{j=0}^{M-1} {f}_{j} {\rm e}^{2\pi{\rm i}\mathbf{k}\mathbf{ x}_j}. \]
\pagebreak

$x^H x$
\pagebreak

$x^H (w \odot x)$
\pagebreak

$x^H (w\odot w2\odot w2 \odot x)$
\pagebreak

$x^H (w2\odot w2 \odot x)$
\pagebreak

$x \leftarrow y$
\pagebreak

$x \leftarrow a y$
\pagebreak

$x \leftarrow w\odot y$
\pagebreak

$x \leftarrow a x + y$
\pagebreak

$x \leftarrow x + a y$
\pagebreak

$x \leftarrow a x + b y$
\pagebreak

$x \leftarrow x + a w\odot y$
\pagebreak

$x \leftarrow a x + w\odot y$
\pagebreak

$[0,1]\times[0,1]{\rm i}$
\pagebreak

$[-1/2,1/2]$
\pagebreak

$2\le\sigma<4$
\pagebreak

$dM$
\pagebreak

$D$
\pagebreak

$N_0+\hdots+N_{d-1}$
\pagebreak

$B$
\pagebreak

$N$
\pagebreak

$\mathbf{x}(m) = \left(x_1,x_2\right) \in [-\frac{1}{2},\frac{1}{2}) \times [0,\frac{1}{2}]$
\pagebreak

$m=0,\ldots, M-1$
\pagebreak

$M \in \mathbb{N},$
\pagebreak

$P_k : \mathbb{R} \rightarrow \mathbb{R}$
\pagebreak

\[ f(x) = \sum_{k=0}^N a_k P_k(x) \quad (N \in \mathbb{N}_0) \]
\pagebreak

\[ P_{k+1}(x) = (alpha_k * x + beta_k)*P_{k}(x) + gamma_k P_{k-1}(x) \quad (alpha_k, beta_k, gamma_k \in \mathbb{R},\; k \ge 0) \]
\pagebreak

$P_{-1}(x) := 0$
\pagebreak

$P_0(x) := \lambda$
\pagebreak

$\left(a_k\right)_{k=0}^N \in \mathbb{C}^{N+1}$
\pagebreak

$\left(x_j\right)_{j=0}^M \in \mathbb{R}^{M+1}$
\pagebreak

$M \in \mathbb{N}_0$
\pagebreak

$\alpha_{k-1}^n$
\pagebreak

$k,n = 0,1,\ldots,N$
\pagebreak

$(N+1)^2$
\pagebreak

$\beta_{k-1}^n$
\pagebreak

$\gamma_{k-1}^n$
\pagebreak

$P_k^n(x,c)$
\pagebreak

$k$
\pagebreak

$\alpha_c^n,\ldots,\alpha_{c+k}^n$
\pagebreak

$\beta_c^n,\ldots,\beta_{c+k}^n$
\pagebreak

$\gamma_c^n,\ldots,\gamma_{c+k}^n$
\pagebreak

$N \in \mathbb{N}_0$
\pagebreak

$\left(b_k^n\right)_{k=0}^M$
\pagebreak

$-M \le n \le M$
\pagebreak

\[ f(\cos\vartheta) = \sum_{k=0}^{2\lfloor\frac{M}{2}\rfloor} a_k (\sin\vartheta)^{n\;\mathrm{mod}\;2} T_k(\cos\vartheta) \]
\pagebreak

$\left(c_k^n\right)_{k=0}^M$
\pagebreak

\[ f(\cos\vartheta) = \sum_{k=-M}^{M} c_k \mathrm{e}^{\mathrm{i}k\vartheta} \]
\pagebreak

$n=-M,\ldots,M$
\pagebreak

$\left(b_k^n\right)_{k=0,\ldots,M;n=-M,\ldots,M}$
\pagebreak

$\left(c_k^n\right)_{k=-M,\ldots,M;n=-M,\ldots,M}$
\pagebreak

$\alpha_l^{km}$
\pagebreak

$m$
\pagebreak

$l$
\pagebreak

$\beta_l^{km}$
\pagebreak

$\gamma_l^{km}$
\pagebreak

$ \alpha_{l}^{km}$
\pagebreak

$ l= 0,\ldots,N $
\pagebreak

$(2N+1)^2(N+1)$
\pagebreak

$ \beta_{l}^{km}$
\pagebreak

$ \gamma_{l}^{km}$
\pagebreak

$ m = -N,\ldots,N $
\pagebreak

$\alpha_{l}^{km}$
\pagebreak

$ k,m = -N,\ldots,N $
\pagebreak

$\beta_{l}^{km}$
\pagebreak

$\gamma_{l}^{km}$
\pagebreak

$d_l^{km}(x,c)$
\pagebreak

$\alpha_c^{km},\ldots,\alpha_{c+l}^{km}$
\pagebreak

$\beta_c^{km},\ldots,\beta_{c+l}^{km}$
\pagebreak

$\gamma_c^{km},\ldots,\gamma_{c+l}^{km}$
\pagebreak

$ d^{km}_l(cos(theta)) $
\pagebreak

$B, B^{\rm T}$
\pagebreak

$\frac{\|x-y\|_{\infty}}{\|x\|_{\infty}} $
\pagebreak

$\frac{\|x-y\|_{\infty}}{\|z\|_1} $
\pagebreak

$\frac{\|x-y\|_2}{\|x\|_2} $
\pagebreak

\[ f(g_q)=\sum^{N}_{l=0}\sum_{m,n=-l}^l \hat f^{mn}_l D_{mn}^l(\alpha_q,\beta_q,\gamma_q) \]
\pagebreak

$[-1/4,1/4]$
\pagebreak

$I_{n+\alpha}(x)$
\pagebreak

$\mathrm{e}^{-x}$
\pagebreak

$x,alpha$
\pagebreak

$0 \le \alpha < 1$
\pagebreak

$n=0,1,\ldots,nb-1$
\pagebreak

$|x| \ge exparg$
\pagebreak

$\min(nb,0)-1$
\pagebreak

$n=0,1,\ldots,ncalc$
\pagebreak

$J_{\nu}(x)$
\pagebreak

$I_{\nu}(x)$
\pagebreak

$x$
\pagebreak

$\nu$
\pagebreak

$\mathbb{R}^3$
\pagebreak

$\mathbb{S}^2$
\pagebreak

$\varphi_1 \in [-\pi,\pi)$
\pagebreak

$\vartheta_1 \in [0,\pi]$
\pagebreak

$\varphi_2 \in [-\pi,\pi)$
\pagebreak

$\vartheta_2 \in [0,\pi]$
\pagebreak

$\cos \vartheta_1 \cos \vartheta_2 + \sin \vartheta_1 \sin(\vartheta_2 \cos(\varphi_1 - \varphi_2)$
\pagebreak

$Q_h: [-1,1] \rightarrow \mathbb{R}$
\pagebreak

$x \in [-1,1]$
\pagebreak

$h \in (0,1)$
\pagebreak

$Q_h(x)$
\pagebreak

$S_h: [-1,1] \rightarrow \mathbb{R}$
\pagebreak

$S_h(x)$
\pagebreak

$L_{h,\lambda}: [-1,1] \rightarrow \mathbb{R}$
\pagebreak

$\lambda \in \mathbb{N}_0$
\pagebreak

$L_{h,\lambda}(x)$
\pagebreak

$G_\sigma: [-1,1] \rightarrow \mathbb{R}$
\pagebreak

$\sigma \in \mathbb{R}_+$
\pagebreak

$G_\sigma(x)$
\pagebreak

$x_{t,j}$
\pagebreak

$w_{t,j}$
\pagebreak

$T$
\pagebreak

$R$
\pagebreak

\[ x_{t,j} := r_j\left(\cos\theta_t, \sin\theta_t\right)^{\top}\,,\qquad (j,t)^{\top}\in I_{\sqrt{2}R}\times I_T\,. \]
\pagebreak

$r_j$
\pagebreak

$\theta_t$
\pagebreak

$M \approx \frac{4}{\pi}\log(1+\sqrt{2}) T R$
\pagebreak

$(j,t)^{\top}\in I_R\times I_T$
\pagebreak

$r_j := \frac{j}{R} \in [-\frac{1}{2},\frac{1}{2})$
\pagebreak

$\theta_t := \frac{\pi t}{T} \in [-\frac{\pi}{2},\frac{\pi}{2})$
\pagebreak

\[ x_{t,j} := r_j\left(\cos\theta_t, \sin\theta_t\right)^{\top}\,. \]
\pagebreak

$M=TR$
\pagebreak

$j \ne 0$
\pagebreak

\[ w_{t,j} = \frac{\pi}{2TR^2}\left(\left(|j|+\frac{1}{2}\right)^2- \left(|j|-\frac{1}{2}\right)^2\right) = \frac{\pi |j| }{TR^2}\, . \]
\pagebreak

$\frac{1}{2R}$
\pagebreak

$\frac{\pi}{4R^2}$
\pagebreak

$w_{t,0} := \frac{\pi}{4TR^2}$
\pagebreak

$\frac{\pi}{4}(1+\frac{1}{R^2})$
\pagebreak

\[ R_{\theta_t} f\left(\frac{s}{R}\right) = \sum_{r \in I_R} w_r \; \sum_{k \in I_N^2} f_{k} \mathrm{e}^{-2\pi\mathrm{I} k \; (\frac{r}{R}\theta_t)} \, \mathrm{e}^{2\pi\mathrm{i} r s / R} \qquad(t \in I_T, s \in I_R). \]
\pagebreak

$\frac{r}{R}\theta_t$
\pagebreak

$w_r$
\pagebreak

$f_k$
\pagebreak

$k \in I_N^2$
\pagebreak

$t \in T$
\pagebreak

\end{document}
